From the Basic Introduction, we thus have

$$
p(x)=\sum_{i=1}^{\infty}C_ix^i
$$

and

$$
p_j(x)=\sum_{i=1}^{\infty}C_{i,j}x^i
$$

as composition won't add a constant element.
Applying composition, we have

$$
p_{j+k}(x)=p_k(p_j(x))=\sum_n C_{n,k}\left(\sum_i C_{i,j} x^i\right)^n=\sum_n\sum_i C_{n,k}\hat B_{i,n}(C_{r,j})x^i
$$

This leads us to the following defining equation:

$$
C_{n,j+k}=\sum_i C_{i,j} \hat B_{n,i}(C_{r,k})=\sum_i C_{i,k} \hat B_{n,i}(C_{r,j})
$$

Taking $k=1$ and the second equality, one can get

$$
C_{N,j}=\frac{1}{C_2(N-2)}\sum_{i=1}^{N-2}\left(C_2C_{i+1,j}C_{N-i,j}+C_{i+2}\hat B_{N+1,i+2}(C_{r,j})-C_{i+1,j}\hat B_{N+1,i+1}(C_r)\right)
$$

This is a way to compute them. A way that I found more useful was to take k=1 and The first equality.

$$
C_{n,j}=\sum_i C_{i,j} \hat B_{n,i}(C_r)
$$

The case $C_1=1$ is especially nice given $C$ 's become polynomial in $j$. This case will thus be studied in its own page.

Staying in the case $C_1\ne1$, here is some examples of $C$'s:

| $i$ | $C_{i,j}$                                                                  |
| --- | -------------------------------------------------------------------------- |
| 1   | $C_1^j$                                                                    |
| 2   | $C_2\frac{C_1^{2j}-C_1^j}{C_1^2-C_1}$                                                            |
| 3   | $\frac{(C_1-1)C_1C_3+2C_2^2}{C_1^2(C_1-1)^2(C_1+1)}C_1^{3j}-\frac{2C_2^2}{(C_1^2-C_1)^2}C_1^{2j}+\frac{(1-C_1)C_3+2C_2^2}{(C_1-1)^2C_1(C_1+1)}C_1^j$                       |

From those, we can guess the model

$$
C_{i,j}=\sum_{k=1}^i C_1^{kj}V_{i,k}(C_r|_{r=1}^i)
$$

Injecting it, we get

$$
\sum_k^iC_{1}^{kj+k}V_{i,k} = \sum_{k=1}^i\sum_{l=k}^i \hat B_{i,l}C_1^{kj}V_{l,k}
$$

which is equivalent to

$$
\sum_{k=1}^iC_1^{kj}\left(C_1^kV_{i,k}-\sum_{l=k}^i \hat B_{i,l} V_{l,k}\right)=0
$$

As this must be true for all $C_1$, we must have

$$
C_1^kV_{i,k}=\sum_{l=k}^i \hat B_{i,l}V_{l,k}
$$

Assuming

$$
\sum_{k=1}^{i}V_{i,k}=0,
$$

we have the following method of computation:

$$
\left\{
	\begin{array}{ll}
	  V_{1,1}=1\\
	  (C_1^k-C_1^i)V_{i,k}=\sum_{l=k}^{i-1}\hat B_{i,l}V_{l,k}\\
	  V_{i,i} = -\sum_{k=1}^{i-1}V_{i,k}
	\end{array}
\right.
$$

The third equations gives us the initial condition of the second one. The first gives the initial condition of the system.
One can see that each $V_i,k$ will introduce a new factor $(C_1^k-C_1^i)^{-1}$ so we have

$$
V_{i,k}\xrightarrow{\prod_{l=k+1}^i(C_1^k-C_1^l)}V_{k,k}V_{i,k}\xrightarrow{\prod_{l=1}^{k-1}(C_1^l-C_1^k)}V_{1,1}=1
$$

We thus can model $V$ as

$$
V_{i,k}=\frac{U_{i,k}}{\prod_{l=1\ne l}^i(C_1^k-C_1^l)}
$$

The second equation then becomes

$$
U_{i,k}=\sum_{l=k}^{i-1}\hat B_{i,l} U_{l,k}\prod_{h=l+1}^{i-1}(C_1^k-C_1^h)
$$

$U$ has the advantage of being a "simple" polynomial and should thus be easier to then model and solve.

| $U_{a,b}$ | b=1 | 2   | 3   |
| --------- | --- | --- | --- |
| a=1       |  $1$   |     |     |
| 2         |  $C_2$   |  $C_2$   |     |
| 3          |  $2C_1C_2^2+C_1(1-C_1)C_3$   |  $2C_1C_2^2$   |  $2C_1C_2^2+C_1^2(C_1-1)C_3$   |

